
@prefix rdf:     <http://www.w3.org/1999/02/22-rdf-syntax-ns#> .
@prefix owl:     <http://www.w3.org/2002/07/owl#> .
@prefix dcterms: <http://purl.org/dc/terms/> .
@prefix xsd:     <http://www.w3.org/2001/XMLSchema#> .
@prefix vann:    <http://purl.org/vocab/vann/> .
@prefix foaf:    <http://xmlns.com/foaf/0.1/> .
@prefix rdfs:    <http://www.w3.org/2000/01/rdf-schema#> .
@prefix qb:      <http://purl.org/linked-data/cube#> .
@prefix daq:     <http://purl.org/eis/vocab/daq#> .
@prefix voaf:    <http://purl.org/vocommons/voaf#> .
@prefix oa:      <http://www.w3.org/ns/oa#> .
@prefix duv:     <http://www.w3.org/ns/duv#> .
@prefix skos:    <http://www.w3.org/2004/02/skos/core#> .
@prefix dqv:      <http://www.w3.org/ns/dqv#> .
@prefix dcat: <http://www.w3.org/ns/dcat#> .
@prefix void: <http://rdfs.org/ns/void#> .
@prefix sdmx-attribute:  <http://purl.org/linked-data/sdmx/2009/attribute#> .
@prefix ex:  <http://example.org/> .



############################
### Metadata section #######
############################
<http://www.w3.org/ns/dqv> a voaf:Vocabulary;
    dcterms:title "Data Quality Vocabulary";
    dcterms:description "The Data Quality Vocabulary (DQV) is seen as an extension to DCAT to cover the quality of the data, how frequently is it updated, whether it accepts user corrections, persistence commitments etc. When used by publishers, this vocabulary will foster trust in the data amongst developers."@en;
    vann:preferredNamespaceUri "http://www.w3.org/ns/dqv";
    vann:preferredNamespacePrefix "dqv";
    foaf:homepage <http://www.w3.org/TR/vocab-dqv/> ;
    dcterms:created "2015-12-17"^^xsd:date;
    dcterms:modified "2015-04-15"^^xsd:date;
    dcterms:publisher <http://www.w3.org/data#W3C>;
    dcterms:type <http://purl.org/adms/assettype/Ontology>;
    dcterms:creator [foaf:name "Antoine Isaac"], [foaf:name "Riccardo Albertoni"] ;
    dcterms:contributor [foaf:name "Jeremy Debattista"], [foaf:name "Makx Dekkers"],  [foaf:name "Christophe Gu√©ret"], [foaf:name "Deirdre Lee"], [foaf:name "Nandana Mihindukulasooriya"], [foaf:name "Amrapali Zaveri"] .


######################
### Classes here #####
######################

dqv:QualityMeasurement a owl:Class, rdfs:Class ;
  rdfs:label "Quality Measurement"@en ;
  rdfs:comment "A quality measurement represents the evaluation of a given dataset (or dataset distribution) against a specific quality metric."@en ;
  owl:equivalentClass daq:Observation;
  rdfs:subClassOf qb:Observation .
  
dqv:Metric a owl:Class, rdfs:Class;
  rdfs:label "Metric"@en ;
  rdfs:comment "A standard to measure a quality dimension. An observation (instance of dqv:QualityMeasurement) assigns a value in a given unit to a Metric."@en ;
  owl:equivalentClass daq:Metric .

dqv:Dimension a owl:Class, rdfs:Class ;
  rdfs:label "Dimension"@en ;
  rdfs:comment "Represents criteria relevant for assessing quality. Each quality dimension must have one or more metric to measure it. A dimension is linked with a category using the dqv:inDimension property."@en ;
  rdfs:subClassOf skos:Concept ;
  owl:equivalentClass daq:Dimension .
  
dqv:Category a owl:Class, rdfs:Class ;
  rdfs:label "Category"@en ;
  rdfs:comment "Represents a group of quality dimensions in which a common type of information is used as quality indicator."@en ;
 rdfs:subClassOf skos:Concept ;
  owl:equivalentClass daq:Category .

dqv:QualityMeasurementDataset a owl:Class, rdfs:Class ;
  rdfs:label "Quality Measurement Dataset"@en ;
  rdfs:comment "Represents a dataset of quality measurements, evaluations of a given dataset (or dataset distribution) against a specific quality metric."@en ;
  rdfs:subClassOf qb:DataSet ;
  owl:equivalentClass daq:QualityGraph .

dqv:QualityPolicy a owl:Class, rdfs:Class ;
  rdfs:label "Quality policy"@en ;
  rdfs:comment "Represents a policy or agreement that is chiefly governed by data quality concerns."@en ;
  .

dqv:QualityAnnotation a owl:Class, rdfs:Class ;
  rdfs:label "Quality Annotation"@en ;
  rdfs:comment "Represents quality annotations, including rating, quality certificate, feedback that can be associated to datasets or distributions. Quality annotations must have one oa:motivatedBy statement with an instance of oa:Motivation (and skos:Concept), which reflects a quality assessment purpose. We define this instance as dqv:qualityAssessment."@en ;
  rdfs:subClassOf oa:Annotation ;
  owl:equivalentClass
    [ rdf:type owl:Restriction ; 
      owl:onProperty oa:motivation ;
      owl:hasValue dqv:qualityAssessment
    ] .

dqv:QualityCertificate a owl:Class, rdfs:Class ;
  rdfs:label "Quality certificate"@en ;
  rdfs:comment "Represents annotations that associate datasets or distributions to quality certificate."@en ;
  rdfs:subClassOf dqv:QualityAnnotation.

dqv:UserQualityFeedback a owl:Class, rdfs:Class ;
  rdfs:label "User Quality feedback"@en ;
  rdfs:comment "Represents feedback users might want to associate to datasets or distributions. Besides dqv:qualityAssessment which is the motivation required by all quality annotations, one of the predefined instances of oa:Motivation should be indicated as motivation to distinguish among the different kinds of feedback, e.g, classifications, questions."@en ;
  rdfs:subClassOf dqv:QualityAnnotation, duv:UserFeedback .

dqv:QualityMetadata a owl:Class, rdfs:Class ;
  rdfs:label "Quality Metadata"@en ;
  rdfs:comment "Represents quality metadata, it is defined to group quality certificates, policies, measurements and annotations under a named graph."@en ;
  rdfs:subClassOf <http://www.w3.org/2004/03/trix/rdfg-1/Graph> ;
  vann:usageNote "QualityMetadata containers do not necessary include all types of quality statements DQV can support. Implementers decide the granularity of containment. In the current version of DQV, we also leave open the choice of the containment technique. Implementers can use (RDF) graph containment. They may also use a dedicated property of their choice to link instances of dqv:QualityMetadata with instances of other DQV classes. For example using (a subproperty of) dcterms:hasPart"@en
.


  
###########################
### Properties here #######
###########################

dqv:isMeasurementOf a rdf:Property, qb:DimensionProperty ;
  rdfs:label "is measurement of"@en ;
  rdfs:comment "Indicates the metric being observed."@en ;
  rdfs:domain qb:Observation ;
  rdfs:range dqv:Metric ;
  owl:equivalentProperty daq:metric .

# this property is still defined in the qb: namespace, the re-definition is therefore commented for now
# dqv:dataSet a rdf:Property ;
#  rdfs:label "data set"@en ;
#  rdfs:comment "Indicates the dataset to a quality measure (which is an RDF Data Cube observation) belongs."@en ;
#  rdfs:domain qb:Observation ;
#  rdfs:range qb:DataSet .

dqv:computedOn a rdf:Property, qb:DimensionProperty ;
  rdfs:label "computed on"@en ;
  rdfs:comment "Refers to the resource (e.g., a dataset, a linkset, a graph, a set of triples) on which the quality measurement is performed. In the DQV context, this property is generally expected to be used in statements in which objects are instances of dcat:Dataset and dcat:Distribution."@en ;
  rdfs:domain dqv:QualityMeasurement ;
  rdfs:range  rdfs:Resource ;
  owl:equivalentProperty daq:computedOn;
  owl:inverseOf dqv:hasQualityMeasurement .

dqv:value a rdf:Property, qb:MeasureProperty, owl:DatatypeProperty ;
  rdfs:label "value"@en ;
  rdfs:comment "Refers to values computed by metric."@en ;
  rdfs:domain dqv:QualityMeasurement ;
  owl:equivalentProperty daq:value .

dqv:expectedDataType a rdf:Property ;
  rdfs:label	"expected data type"@en ;
  rdfs:comment "Represents the expected data type for metric's observed value (e.g. xsd:boolean, xsd:double etc...)"@en ;
  rdfs:domain dqv:Metric ;
  rdfs:domain xsd:anySimpleType ;
  owl:equivalentProperty daq:expectedDataType .

dqv:inCategory a rdf:Property ;
  rdfs:label "in category"@en ;
  rdfs:comment "Represents the category a dimension is grouped in."@en ;
  rdfs:domain dqv:Dimension ;
  rdfs:range dqv:Category ;
  owl:inverseOf daq:hasDimension ;
  vann:usageNote "Categories are meant to systematically organize dimensions. The Data Quality Vocabulary defines no specific cardinality constraints for dqv:inCategory, since distinct quality frameworks might have different perspectives over a dimension. A dimension may therefore be associated to more than one category. However, those who define new quality metrics should try to avoid this as much as possible and assign only one category to the dimensions they define."@en .

dqv:inDimension a rdf:Property ;
  rdfs:label "in dimension"@en ;
  rdfs:comment "Represents the dimension a metric allows a measurement of."@en ;
  rdfs:range dqv:Dimension ;
 ## to add the equivalence  to SubObjectPropertyOf( ObjectInverseOf( daq:hasMetric )  dqv:inDimension)                           
  vann:usageNote "Dimensions are meant to systematically organize metrics. The Data Quality Vocabulary define no specific cardinality constraints for dqv:hasDimension, since distinct quality frameworks might have different perspectives over a metric. A metric may therefore be associated to more than one dimension. However, those who define new quality measures should try to avoid this as much as possible and assign only one dimension to the metrics they define."@en .


dqv:hasQualityMeasurement a rdf:Property ;
  rdfs:label "has quality measurement"@en ;
  rdfs:comment "Refers to the performed quality measurements. Quality measurements can be performed to any kind of resource (e.g., a dataset, a linkset, a graph, a set of triples). However, in the DQV context, this property is generally expected to be used in statements in which subjects are instances of dcat:Dataset and dcat:Distribution."@en ;
  rdfs:range dqv:QualityMeasurement ;
  owl:inverseOf dqv:computedOn .


###########################
### Instances here #######
###########################

dqv:qualityAssessment a oa:Motivation ;
  skos:prefLabel "Quality assessment"@en ;
  skos:definition "Motivation that must be specified for quality annotations"@en ;
  skos:closeMatch oa:moderating .

dqv:precision a oa:Motivation ;
  skos:prefLabel "Precision"@en ;
  skos:definition "Precision is a quality dimension which refers to the recorded level of details. It represents the exactness of measurement or description."@en 
.



#########################################################
##########################¬†EXAMPLE #######################
#########################################################

### Dataset and Linkset
ex:myDataset1 
    a dcat:Dataset ;
    dcterms:title "My dataset 1" 
    .

ex:myDataset2 
    a dcat:Dataset ;
    dcterms:title "My dataset 2"  
    .

ex:myLinkset 
    a dcat:Dataset, void:Linkset ;
    dcterms:title "A Linkset between My dataset 1 and My dataset 2"; 
    void:linkPredicate skos:exactMatch ;
    void:target ex:myDataset1 ;
    void:target ex:myDataset2  
    .

# Definition of instances for Metric, Dimension and Category. 

ex:importingForPropertyPercentage 
    a dqv:Metric ;
    skos:definition "Ratio between novel preferred or alternative labels gained via skos:exactMatch links and preferred or alternative labels already in the dataset."@en ;
    dqv:expectedDataType xsd:double ;
    dqv:inDimension  ex:completeness .

ex:completenessGain
    a  dqv:Dimension ;
    skos:prefLabel "Completeness Gain"@en ;
    skos:definition "Degree to which a linkset contributes to obtaining all required information in a particular dataset."@en ;
    dqv:inCategory ex:complementationGain 
    .

ex:complementationGain
    a  dqv:Category ;
    skos:definition "Category that groups dimensions measuring the data quality gain  obatined by exploiting linksets."@en
    .

ex:onLanguage
    a qb:DimensionProperty, owl:DataProperty ;
    rdfs:comment   "language on which label importing is assessed."@en ;
    rdfs:domain    dqv:QualityMeasurement;
    rdfs:range       xsd:string ;
    rdfs:label     "label import assessment language"@en 
    .

ex:onProperty
    a qb:DimensionProperty, rdf:Property ;
    rdfs:comment 	"property on which label importing is assessed."@en ;
    rdfs:domain 	dqv:QualityMeasurement ;
    rdfs:label  	"label import assessment property"@en ;
    rdfs:range     	rdf:Property 
    .
        

#####Quality Assessment
ex:qualityMeasurementDataset  a  dqv:QualityMeasurementDataset ;
        qb:structure  ex:dsd .

ex:importingForPropertyPercentage
    dqv:hasObservation ex:measurement_exactMatchAltLabelItDataset1,
    ex:measurement_exactMatchAltLabelItDataset2, 
    ex:measurement_exactMatchAltLabelEnDataset1, 
    ex:measurement_exactMatchAltLabelEnDataset2,
    ex:measurement_exactMatchPrefLabelItDataset1, 
    ex:measurement_exactMatchprefLabelItDataset2 .


#Adding quality observations 
## for Italian alternative labels
ex:measurement_exactMatchAltLabelItDataset1 
       a 		dqv:QualityMeasurement;
       dqv:computedOn  	ex:myLinkset ;
       dqv:value       	"1.0"^^xsd:double ;
       dcterms:date          "2016-01-10"^^xsd:date  ;
       dqv:isMeasurementOf      	ex:importingForPropertyPercentage ;
       qb:dataSet      	ex:qualityMeasurementDataset;
       ex:onLanguage    	"it" ;
       ex:onProperty    	skos:altLabel .

ex:measurement_exactMatchAltLabelItDataset2 
       a 		dqv:QualityMeasurement;
       dqv:computedOn  	ex:myLinkset ;
       dqv:value       	"1.0"^^xsd:double ;
       dcterms:date          "2016-03-10"^^xsd:date  ;
       dqv:isMeasurementOf      	ex:importingForPropertyPercentage ;
       qb:dataSet      	ex:qualityMeasurementDataset;
       ex:onLanguage    	"it" ;
       ex:onProperty    	skos:altLabel .

## for English alternative labels
ex:measurement_exactMatchAltLabelEnDataset1 
       a 		dqv:QualityMeasurement;
       dqv:computedOn  	ex:myLinkset ;
       dqv:value       	"0.1"^^xsd:double ;
       dcterms:date          "2016-01-10"^^xsd:date  ;
       dqv:isMeasurementOf      	ex:importingForPropertyPercentage ;
       qb:dataSet      	ex:qualityMeasurementDataset;
       ex:onLanguage    	"en" ;
       ex:onProperty    	skos:altLabel .

ex:measurement_exactMatchAltLabelEnDataset2  
       a 		dqv:QualityMeasurement;
       dqv:computedOn  	ex:myLinkset ;
       dqv:value       	"1.0"^^xsd:double ;
       dcterms:date          "2016-03-10"^^xsd:date  ;
       dqv:isMeasurementOf      	ex:importingForPropertyPercentage ;
       qb:dataSet      	ex:qualityMeasurementDataset;
       ex:onLanguage    	"en" ;
       ex:onProperty    	skos:altLabel .      

## for Italian preferred labels
ex:measurement_exactMatchPrefLabelItDataset1 
       a 		dqv:QualityMeasurement;
       dqv:computedOn  	ex:myLinkset ;
       dqv:value       	"0.5"^^xsd:double ;
       dcterms:date          "2016-01-10"^^xsd:date  ;
       dqv:isMeasurementOf      	ex:importingForPropertyPercentage ;
       qb:dataSet      	ex:qualityMeasurementDataset;
       ex:onLanguage    	"it" ;
       ex:onProperty    	skos:prefLabel .

ex:measurement_exactMatchprefLabelItDataset2  
       a 		dqv:QualityMeasurement;
       dqv:computedOn  	ex:myLinkset ;
       dqv:value       	"0.5"^^xsd:double ;
       dqv:isMeasurementOf      	ex:importingForPropertyPercentage ;
       qb:dataSet      	ex:qualityMeasurementDataset;
       ex:onLanguage    	"it" ;
       dcterms:date          "2016-03-10"^^xsd:date  ;
       ex:onProperty    	skos:prefLabel .


ex:dsd  a     qb:DataStructureDefinition ;
##Copying the structure of daq:dsq
 ##the dimensions
    qb:component  [ qb:dimension  dqv:computedOn ;
                    qb:order      2
                  ] ;
    qb:component  [ qb:dimension       dcterms:date;
                    qb:order      3
                  ] ;
    qb:component  [ qb:dimension  dqv:isMeasurementOf ;
                    qb:order      1
                  ] ;
    #The measure
   qb:component  [ qb:measure  dqv:value ; ] ;


    # Attribute (here: unit of measurement)
    qb:component [
        qb:attribute sdmx-attribute:unitMeasure
    ;
    qb:componentRequired false ;
    qb:componentAttachment qb:DataSet ; ] ;


    ##Extending  the structure of lds:dsq with two new dimensions
    qb:component  [ qb:dimension  ex:onProperty ;
                    qb:order      4
                  ] ;
    qb:component  [ qb:dimension  ex:onLanguage ;
                    qb:order      5
                  ] .

######### Adding dataset #######
ex:qualityMeasurementDataset a qb:DataSet;
    rdfs:label "Linkset quality"@en;
    rdfs:comment "Example of linkset quality DQV encoding"@en;
    qb:structure ex:dsd  
    .  

###########################
#### Using the validator http://computex.herokuapp.com/
### All the properties that are dimensions must have  a range  --- > so we need to add rage for onProperty onLanguage, and also dqv:value dqv:computedOn
### two observations in the same cube can't have the same value for all dimensions ---> so we need to add the  dimension dcterms:date in the data cube structure, 

<http://purl.org/dc/terms/date> rdfs:range xsd:date.

#### Perhaps we should add also info about qb:dataSet, if we want to make this example browsable for example by http://km.aifb.kit.edu/projects/ldcx/ 
